Exercises/ex8.lean
@@ -1,0 +1,105 @@
+-- Open a namespace Hidden to avoid naming conflicts, and use the equation compiler to define addition, multiplication, and exponentiation on the natural numbers. Then use the equation compiler to derive some of their basic properties.
+namespace Hidden
+--ex 1
+@[simp] def add : Nat → Nat → Nat
+| 0, b => b
+| a + 1, b => add a b + 1
+@[simp] def mul : Nat → Nat → Nat
+| 0, _ => 0
+| a + 1, b => add (mul a b) b
+@[simp] def exp : Nat → Nat → Nat
+| _, 0 => 1
+| a, b +1 => mul a (exp a b)
+theorem add_zero : ∀ a, add a 0 = a
+  | Nat.zero => rfl
+  | Nat.succ a => congrArg Nat.succ (add_zero a)
+theorem mul_1 : ∀ a, mul 1 a = a
+  | Nat.zero => rfl
+  | a + 1 => by simp[mul, add]
+theorem exp_0 : ∀ a, exp 1 a = 1
+  | Nat.zero => rfl
+  | Nat.succ a => by simp[exp_0 a]
+
+--ex 2
+
+def reverse : List α → List α
+| [] => []
+| x :: xs => reverse xs ++ [x]
+theorem reverse_reverse : ∀ xs : List α, reverse (reverse xs) = xs := by
+  intro xs
+  induction xs with
+  | nil => rfl
+  | cons x xs ih => simp [reverse,reverse_append, List.nil_append,List.singleton_append,ih]
+where
+  reverse_append (as bs: List α) : reverse (as ++ bs) = reverse bs ++ reverse as := by
+    induction as with
+    | nil => rw [reverse, List.nil_append, List.append_nil]
+    | cons a as' ih =>
+      simp [List.cons_append, reverse, ih, List.append_assoc]
+
+#print reverse
+
+--ex 4
+open  Nat
+inductive Vector (α : Type u) : Nat → Type u
+  | nil  : Vector α 0
+  | cons : α → {n : Nat} → Vector α n → Vector α (n+1)
+
+#eval  Vector.cons 5 Vector.nil
+
+def append {α : Type u} {n m : Nat} : Vector α n → Vector α m → Vector α (n + m)
+  | Vector.nil,        ys => by
+    simp [Nat.zero_add]
+    exact ys
+  | Vector.cons x xs,  ys => by
+    simp [Nat.succ_add]
+    exact
+    Vector.cons x (append xs ys)
+
+--ex 5
+inductive Expr where
+  | const : Nat → Expr
+  | var : Nat → Expr
+  | plus : Expr → Expr → Expr
+  | times : Expr → Expr → Expr
+  deriving Repr
+
+open Expr
+
+def sampleExpr : Expr :=
+  plus (times (var 0) (const 7)) (times (const 2) (var 1))
+
+def eval (v : Nat → Nat) : Expr → Nat
+  | const n     => n
+  | var n       => v n
+  | plus e₁ e₂  => eval v e₁ + eval v e₂
+  | times e₁ e₂ => eval v e₁ * eval v e₂
+
+def sampleVal : Nat → Nat
+  | 0 => 5
+  | 1 => 6
+  | _ => 0
+
+#eval eval sampleVal sampleExpr --47
+
+def simpConst : Expr → Expr
+  | plus (const n₁) (const n₂)  => const (n₁ + n₂)
+  | times (const n₁) (const n₂) => const (n₁ * n₂)
+  | e                           => e
+
+def fuse : Expr → Expr
+  | plus e₁ e₂  => simpConst (plus (fuse e₁) (fuse e₂))
+  | times e₁ e₂ => simpConst (times (fuse e₁) (fuse e₂))
+  | e => e
+
+theorem simpConst_eq (v : Nat → Nat) : ∀ (e : Expr), eval v (simpConst e) = eval v e
+  | plus e1 e2 => by cases e1 <;> cases e2 <;> rfl
+  | times e1 e2 => by cases e1 <;> cases e2 <;> rfl
+  | var x => rfl
+  | const n => rfl
+
+theorem fuse_eq (v : Nat → Nat) : ∀ e : Expr, eval v (fuse e) = eval v e
+  | const n     => rfl
+  | var n       => rfl
+  | plus e₁ e₂  => by rw [fuse,simpConst_eq,eval,eval,fuse_eq,fuse_eq]
+  | times e₁ e₂ => by rw [fuse,simpConst_eq,eval,eval,fuse_eq,fuse_eq]
